theories/RTac/Idtac.v
@@ -3,7 +3,6 @@ Require Import MirrorCore.EnvI.
 Require Import MirrorCore.ExprI.
 Require Import MirrorCore.TypesI.
 Require Import MirrorCore.SubstI.
-Require Import MirrorCore.ExprDAs.
 Require Import MirrorCore.RTac.Core.
 
 Require Import MirrorCore.Util.Forwardy.
@@ -22,30 +21,17 @@ Section parameterized.
   Variable Subst_subst : Subst subst expr.
   Variable SubstOk_subst : @SubstOk _ _ _ _ Expr_expr Subst_subst.
 
-  Definition THEN (c1 c2 : rtac typ expr subst) : rtac typ expr subst :=
-    fun gl =>
-      match c1 gl with
-        | Some gl' => c2 gl'
-        | None => None
-      end.
+  Definition IDTAC : rtac typ expr subst :=
+    fun gl => Some gl.
 
-  Theorem THEN_sound
-  : forall (tus tvs : list typ) (tac1 tac2 : rtac typ expr subst),
-      rtac_sound tus tvs tac1 ->
-      rtac_sound tus tvs tac2 ->
-      rtac_sound tus tvs (THEN tac1 tac2).
+  Theorem IDTAC_sound
+  : forall tus tvs, rtac_sound tus tvs IDTAC.
   Proof.
-    unfold THEN.
+    unfold IDTAC, rtac_sound.
     intros.
-    red. intros.
-    forward.
-    eapply H in H1; clear H.
-    eapply H1 in H2; clear H1.
-    destruct H2.
-    eapply H0 in H3; eauto.
-    specialize (H3 H). forward_reason.
+    inv_all; subst.
     split; auto.
-    forward. eauto.
+    forward.
   Qed.
 
 End parameterized.
